Improved the efficiency of some tactics and finished formalising the refinement of Sqrt.

Sqrt.v
@@ -25,13 +25,153 @@ Definition find_eqb_some (h : option nat) : nat :=
     | _ => 0
   end.
 
+Definition lift_opt_prop {a} (f : a -> a -> Prop) (v1 : option a) (v2 : option a) : Prop :=
+  match v1,v2 with
+    | Some x, Some y => f x y
+    | _, _ => False
+  end.
+
+Definition Inv (Q R : Ptr) (s : nat) (si st : heap nat) :=
+    prod (lift_opt_prop (fun r s => Nat.le (square r) s) (find st R) (Some s))
+    (prod (lift_opt_prop (fun s q => Nat.lt s (square q)) (Some s) (find st Q)) (R <> Q)).
+
+Definition Cond (Q R : Ptr) (st : heap nat) :=
+  negb (Nat.eqb (find_eqb_some (find st R) + 1)
+                (find_eqb_some (find st Q))).
+
+Definition sqrt (ptr : Ptr) : WhileL nat nat.
+refine (
+  Read ptr (fun s =>
+  New (s + 1) (fun Q =>
+  New 0 (fun R =>
+  While (Inv Q R s)
+        (Cond Q R)
+        (Read Q (fun vInQ =>
+        (Read R (fun vInR =>
+        let p := div2 (vInQ + vInR)
+        in if (s <? square p)
+           then Write Q p (Return _ tt)
+           else Write R p (Return _ tt)))))
+  (Read R (fun vInR => Return _ vInR)))))).
+Defined.
+
+Lemma sqrtRefinement : forall ptr, wrefines (sqrtSpec ptr) (sqrt ptr).
+Proof.
+  intro ptr; unfold sqrtSpec.
+  READ ptr s.
+  NEW (s + 1) Q.
+  NEW 0 R.
+  unfold Inv, Cond; apply whileSpec.
+  - refine_simpl.
+    unfold lift_opt_prop, square; simpl; rewrite findUpdate; simpl; apply le_0_n.
+    unfold square; simpl; rewrite findNUpdate.
+    unfold Nat.lt; rewrite findUpdate; simpl.
+    remember ((s + 1) * (s + 1)).
+    rewrite Nat.add_comm in Heqn1 at 1; simpl in Heqn1.
+    rewrite Nat.add_comm with (m := 1) in Heqn1; rewrite Heqn1.
+    apply Nat.le_add_r.
+    unfold not; intro H'; subst.
+    assert (Ha : R <> R) by eauto; now apply Ha.
+    unfold not; intro H'; subst.
+    assert (Ha : Q <> Q) by eauto; now apply Ha.
+  - READ Q vInQ.
+    remember (find s0 Q).
+    destruct o; [ eauto | exfalso; assumption ].
+    READ R vInR.
+    unfold lift_opt_prop in l.
+    remember (find s0 R) as r; destruct r; [ eauto | exfalso; assumption ].
+    remember (s <? square (Nat.div2 (vInQ + vInR))) as b.
+    destruct b.
+    WRITE Q (Nat.div2 (vInQ + vInR)).
+    RETURN tt;
+    try rewrite findUpdate; try rewrite findNUpdate; auto.
+    rewrite e1 in y; rewrite e0 in l; symmetry in Heqb; now apply Nat.ltb_lt.
+    WRITE R (Nat.div2 (vInQ + vInR)).
+    RETURN tt;
+    try rewrite findUpdate; try rewrite findNUpdate; auto.
+    simpl; symmetry in Heqb; apply leb_iff_conv in Heqb;
+    now apply Lt.lt_n_Sm_le in Heqb.
+  - READ R vInR.
+    unfold lift_opt_prop in l.
+    remember (find s0 R) as r; destruct r; [ eauto | exfalso; assumption ].
+    RETURN vInR.
+    * rewrite e in l; simpl in l; auto.
+    * rewrite e in i; simpl in i.
+      remember (find s0 Q) as q; destruct q.
+      remember (vInR + 1 =? n2) as b; destruct b.
+      apply beq_nat_eq in Heqb.
+      now subst.
+      exfalso; simpl in i; rewrite <- Heqb in i; auto.
+      exfalso; assumption.
+Qed.
+
+Lemma ifSpec {a v} (cond : bool) (spec : PT v a) (wt we : WhileL v a) :
+  (if cond then Spec spec ⊑ wt else Spec spec ⊑ we) ->
+  (Spec spec ⊑ (if cond then wt else we)).
+Proof. destruct cond; intros; assumption. Qed.
+
+Definition sqrtResult (ptr : Ptr) :
+  {c : WhileL nat nat & sqrtSpec ptr ⊑ c}.
+Proof.
+  econstructor; unfold sqrtSpec.
+  READ ptr s.
+  NEW (s + 1) Q.
+  NEW 0 R.
+  apply whileSpec with (I := Inv Q R s) (c := Cond Q R); unfold Inv, Cond.
+  - refine_simpl.
+    unfold lift_opt_prop, square; simpl; rewrite findUpdate; simpl; apply le_0_n.
+    unfold square; simpl; rewrite findNUpdate.
+    unfold Nat.lt; rewrite findUpdate; simpl.
+    remember ((s + 1) * (s + 1)).
+    rewrite Nat.add_comm in Heqn1 at 1; simpl in Heqn1.
+    rewrite Nat.add_comm with (m := 1) in Heqn1; rewrite Heqn1.
+    apply Nat.le_add_r.
+    unfold not; intro H'; subst; assert (Ha : R <> R) by eauto; now apply Ha.
+    unfold not; intro H'; subst; assert (Ha : Q <> Q) by eauto; now apply Ha.
+  - READ Q vInQ.
+    remember (find s0 Q) as o.
+    destruct o; [ eauto | exfalso; assumption ].
+    READ R vInR.
+    unfold lift_opt_prop in l.
+    remember (find s0 R) as r; destruct r; [ eauto | exfalso; assumption ].
+    remember (s <? square (Nat.div2 (vInQ + vInR))) as b.
+    apply ifSpec with (cond := s <? square (Nat.div2 (vInQ + vInR))).
+    destruct b; rewrite <- Heqb; simpl.
+    (* WRITE Q (Nat.div2 (vInQ + vInR)). *)
+    eapply (@writeSpec _ _ Q (Nat.div2 (vInQ + vInR))).
+    intros; simpl in *; destruct_conjs'; eexists; apply e0.
+    RETURN tt; try rewrite findUpdate; try rewrite findNUpdate; auto.
+    rewrite e1 in y; rewrite e0 in l; symmetry in Heqb; now apply Nat.ltb_lt.
+    (* WRITE R (Nat.div2 (vInQ + vInR)). *)
+    eapply (@writeSpec _ _ R (Nat.div2 (vInQ + vInR))).
+    intros; simpl in *; destruct_conjs'; eexists; apply e.
+    RETURN tt;
+    try rewrite findUpdate; try rewrite findNUpdate; auto.
+    simpl; symmetry in Heqb; apply leb_iff_conv in Heqb;
+    now apply Lt.lt_n_Sm_le in Heqb.
+  - READ R vInR.
+    unfold lift_opt_prop in l.
+    remember (find s0 R) as r; destruct r; [ eauto | exfalso; assumption ].
+    RETURN vInR.
+    * rewrite e in l; simpl in l; auto.
+    * rewrite e in i; simpl in i.
+      remember (find s0 Q) as q; destruct q.
+      remember (vInR + 1 =? n2) as b; destruct b.
+      apply beq_nat_eq in Heqb.
+      now subst.
+      exfalso; simpl in i; rewrite <- Heqb in i; auto.
+      exfalso; assumption.  
+Qed.
+
+(* Refinement with Type *)
+
 Definition lift_opt {a b} (f : a -> a -> b) (v1 : option a) (v2 : option a) : option b :=
   match v1,v2 with
     | Some x, Some y => Some (f x y)
     | _, _ => None
   end.
 
-Definition sqrt (ptr : Ptr) : WhileL nat nat.
+Definition sqrt_type (ptr : Ptr) : WhileL nat nat.
 refine (
   Read ptr (fun s =>
   New (s + 1) (fun Q =>
@@ -50,22 +190,12 @@ refine (
   (Read R (fun vInR => Return _ vInR)))))).
 Defined.
 
-(* This is so slow that I can't even get past the first READ
-Definition sqrtResult (ptr : Ptr) :
-  {c : WhileL nat nat & sqrt ptr ⊑ c}.
-Proof.
-  econstructor; unfold sqrt.
-  eapply readSpec.
-  READ ptr s.
-Qed.  
-*)
-
-Lemma sqrtRefinement : forall ptr, wrefines (sqrtSpec ptr) (sqrt ptr).
+Lemma sqrtRefinement_type : forall ptr, wrefines (sqrtSpec ptr) (sqrt_type ptr).
 Proof.
   intro ptr; unfold sqrtSpec.
   READ ptr s.
-  apply newSpec'; intro Q.
-  apply newSpec'; intro R.
+  NEW (s + 1) Q.
+  NEW 0 R.
   apply whileSpec.
   - refine_simpl.
     unfold lift_opt, square; simpl; rewrite findUpdate; now simpl.
